ByteFile.v: export bytefile-specific file attributes
This is basically INODE.iattr minus the file length.  Useful for
concisely stating that file attributes are preserved even if the
bytefile is resized.

XXX need to go back and fix up proofs.

src/ByteFile.v
@@ -44,6 +44,12 @@ Module BYTEFILE.
     reflexivity.
   Qed.
 
+  Record bytefile_attr := {
+    FMTime : word 32;
+    FType : word 32;
+    FDev : word 64
+  }.
+
   (* The bytes of a file are mapped onto a list of blocks:   *)
   (*   [ block 0 ... block n]                                *)
   (*   <-- allbytes      -->                                 *)
@@ -53,12 +59,15 @@ Module BYTEFILE.
     BFileRec.array_item_file byte_type items_per_valu itemsz_ok f allbytes /\
     # (natToWord addrlen (length allbytes)) = length allbytes.
 
-  Definition rep (bytes : list byte) (f : BFILE.bfile) :=
+  Definition rep (bytes : list byte) (attr : bytefile_attr) (f : BFILE.bfile) :=
     exists allbytes,
     bytes_rep f allbytes /\
     firstn (# (f.(BFILE.BFAttr).(INODE.ISize))) allbytes = bytes /\
     length bytes = (# (f.(BFILE.BFAttr).(INODE.ISize))) /\
-    divup # (INODE.ISize (BFILE.BFAttr f)) valubytes * valubytes = length allbytes.
+    divup # (INODE.ISize (BFILE.BFAttr f)) valubytes * valubytes = length allbytes /\
+    FMTime attr = INODE.IMTime (BFILE.BFAttr f) /\
+    FType attr = INODE.IType (BFILE.BFAttr f) /\
+    FDev attr = INODE.IDev (BFILE.BFAttr f).
 
   Lemma block_items_ok : block_items items_per_valu = valubytes.
   Proof.
@@ -159,11 +168,11 @@ Module BYTEFILE.
   Qed.
 
   Theorem read_bytes_ok: forall fsxp inum off len mscs,
-  {< m mbase F Fm A flist f bytes,
+  {< m mbase F Fm A flist f bytes attr,
   PRE LOG.rep (FSXPLog fsxp) F (ActiveTxn mbase m) mscs *
       [[ (Fm * BFILE.rep (FSXPBlockAlloc fsxp) (FSXPInode fsxp) flist)%pred (list2mem m) ]] *
       [[ (A * #inum |-> f)%pred (list2nmem flist) ]] *
-      [[ rep bytes f ]]
+      [[ rep bytes attr f ]]
    POST RET:^(mscs, b)
       exists Fx v,
       LOG.rep (FSXPLog fsxp) F (ActiveTxn mbase m) mscs *
@@ -237,11 +246,11 @@ Module BYTEFILE.
   Hint Extern 1 ({{_}} progseq (read_bytes _ _ _ _ _) _) => apply read_bytes_ok : prog.
 
   Theorem update_bytes_ok: forall fsxp inum off len (newbytes : bytes len) mscs,
-      {< m mbase F Fm A flist f bytes olddata Fx,
+      {< m mbase F Fm A flist f bytes attr olddata Fx,
        PRE LOG.rep (FSXPLog fsxp) F (ActiveTxn mbase m) mscs *
            [[ (Fm * BFILE.rep (FSXPBlockAlloc fsxp) (FSXPInode fsxp) flist)%pred (list2mem m) ]] *
            [[ (A * #inum |-> f)%pred (list2nmem flist) ]] *
-           [[ rep bytes f ]] *
+           [[ rep bytes attr f ]] *
            [[ (Fx * arrayN off olddata)%pred (list2nmem bytes) ]] *
            [[ length olddata = len ]]
       POST RET: ^(mscs)
@@ -249,10 +258,9 @@ Module BYTEFILE.
            LOG.rep (FSXPLog fsxp) F (ActiveTxn mbase m') mscs *
            [[ (Fm * BFILE.rep (FSXPBlockAlloc fsxp) (FSXPInode fsxp) flist')%pred (list2mem m') ]] *
            [[ (A * #inum |-> f')%pred (list2nmem flist') ]] *
-           [[ rep bytes' f' ]] *
+           [[ rep bytes' attr f' ]] *
            [[ let newdata := @Rec.of_word (Rec.ArrayF byte_type len) newbytes in
-              (Fx * arrayN off newdata)%pred (list2nmem bytes') ]] *
-           [[ hidden (BFILE.BFAttr f = BFILE.BFAttr f') ]]
+              (Fx * arrayN off newdata)%pred (list2nmem bytes') ]]
        CRASH LOG.would_recover_old (FSXPLog fsxp) F mbase
       >} update_bytes fsxp inum off newbytes mscs.
   Proof.
@@ -349,11 +357,11 @@ Module BYTEFILE.
   Definition filelen f := # (INODE.ISize (BFILE.BFAttr f)).
 
   Theorem grow_file_ok: forall fsxp inum newlen mscs,
-    {< m mbase F Fm A flist f bytes,
+    {< m mbase F Fm A flist f bytes attr,
       PRE LOG.rep (FSXPLog fsxp) F (ActiveTxn mbase m) mscs *
            [[ (Fm * BFILE.rep (FSXPBlockAlloc fsxp) (FSXPInode fsxp) flist)%pred (list2mem m) ]] *
            [[ (A * #inum |-> f)%pred (list2nmem flist) ]] *
-           [[ rep bytes f ]] *
+           [[ rep bytes attr f ]] *
            [[ goodSize addrlen newlen ]] *
            (* spec requires that file is growing, so that it can guarantee
               that the new size of the file is $newlen. *)
@@ -361,13 +369,13 @@ Module BYTEFILE.
       POST RET:^(mscs, ok)
            exists m', LOG.rep (FSXPLog fsxp) F (ActiveTxn mbase m') mscs *
            ([[ ok = false ]] \/
-           [[ ok = true ]] * exists flist' f' bytes' fdata' attr,
+           [[ ok = true ]] * exists flist' f' bytes' fdata' fattr',
            [[ (Fm * BFILE.rep (FSXPBlockAlloc fsxp) (FSXPInode fsxp) flist')%pred (list2mem m') ]] *
            [[ (A * #inum |-> f')%pred (list2nmem flist') ]] *
            [[ bytes' = (bytes ++ (repeat $0 (newlen -  (# (INODE.ISize (BFILE.BFAttr f)))))) ]] *
-           [[ rep bytes' f' ]] *
-           [[ attr = INODE.Build_iattr ($ newlen) f.(BFILE.BFAttr).(INODE.IMTime) f.(BFILE.BFAttr).(INODE.IType) f.(BFILE.BFAttr).(INODE.IDev) ]] *
-           [[ f' = BFILE.Build_bfile fdata' attr ]])
+           [[ rep bytes' attr f' ]] *
+           [[ fattr' = INODE.Build_iattr ($ newlen) f.(BFILE.BFAttr).(INODE.IMTime) f.(BFILE.BFAttr).(INODE.IType) f.(BFILE.BFAttr).(INODE.IDev) ]] *
+           [[ f' = BFILE.Build_bfile fdata' fattr' ]])
        CRASH LOG.would_recover_old (FSXPLog fsxp) F mbase
      >} grow_file fsxp inum newlen mscs.
    Proof.
@@ -555,23 +563,23 @@ Module BYTEFILE.
     }.
 
   Theorem shrink_file_ok: forall fsxp inum newlen mscs,
-    {< m mbase F Fm A flist f bytes,
+    {< m mbase F Fm A flist f bytes attr,
       PRE LOG.rep (FSXPLog fsxp) F (ActiveTxn mbase m) mscs *
            [[ (Fm * BFILE.rep (FSXPBlockAlloc fsxp) (FSXPInode fsxp) flist)%pred (list2mem m) ]] *
            [[ (A * #inum |-> f)%pred (list2nmem flist) ]] *
-           [[ rep bytes f ]] *
+           [[ rep bytes attr f ]] *
            [[ goodSize addrlen newlen ]] *
            [[ newlen <= filelen f ]]
       POST RET:^(mscs, ok)
            exists m', LOG.rep (FSXPLog fsxp) F (ActiveTxn mbase m') mscs *
            ([[ ok = false ]] \/
-           [[ ok = true ]] * exists flist' f' bytes' fdata' attr,
+           [[ ok = true ]] * exists flist' f' bytes' fdata' fattr',
            [[ (Fm * BFILE.rep (FSXPBlockAlloc fsxp) (FSXPInode fsxp) flist')%pred (list2mem m') ]] *
            [[ (A * #inum |-> f')%pred (list2nmem flist') ]] *
            [[ bytes' = firstn newlen bytes ]] *
-           [[ rep bytes' f' ]] *
-           [[ attr = INODE.Build_iattr ($ newlen) f.(BFILE.BFAttr).(INODE.IMTime) f.(BFILE.BFAttr).(INODE.IType) f.(BFILE.BFAttr).(INODE.IDev) ]] *
-           [[ f' = BFILE.Build_bfile fdata' attr ]])
+           [[ rep bytes' attr f' ]] *
+           [[ fattr' = INODE.Build_iattr ($ newlen) f.(BFILE.BFAttr).(INODE.IMTime) f.(BFILE.BFAttr).(INODE.IType) f.(BFILE.BFAttr).(INODE.IDev) ]] *
+           [[ f' = BFILE.Build_bfile fdata' fattr' ]])
        CRASH LOG.would_recover_old (FSXPLog fsxp) F mbase
      >} shrink_file fsxp inum newlen mscs.
   Proof.
@@ -631,8 +639,8 @@ Module BYTEFILE.
   Hint Extern 1 ({{_}} progseq (shrink_file _ _ _ _) _) => apply shrink_file_ok : prog.
 
 
-  Lemma rep_length : forall bytes f,
-    rep bytes f ->
+  Lemma rep_length : forall bytes attr f,
+    rep bytes attr f ->
     length bytes = (# (f.(BFILE.BFAttr).(INODE.ISize))).
   Proof.
     unfold rep. intuition deex.
@@ -657,22 +665,22 @@ Module BYTEFILE.
     }.
 
   Theorem resize_file_ok: forall fsxp inum newlen mscs,
-    {< m mbase F Fm A flist f bytes,
+    {< m mbase F Fm A flist f bytes attr,
       PRE LOG.rep (FSXPLog fsxp) F (ActiveTxn mbase m) mscs *
            [[ (Fm * BFILE.rep (FSXPBlockAlloc fsxp) (FSXPInode fsxp) flist)%pred (list2mem m) ]] *
            [[ (A * #inum |-> f)%pred (list2nmem flist) ]] *
-           [[ rep bytes f ]] *
+           [[ rep bytes attr f ]] *
            [[ goodSize addrlen newlen ]]
       POST RET:^(mscs, ok)
            exists m', LOG.rep (FSXPLog fsxp) F (ActiveTxn mbase m') mscs *
            ([[ ok = false ]] \/
-           [[ ok = true ]] * exists flist' f' bytes' fdata' attr,
+           [[ ok = true ]] * exists flist' f' bytes' fdata' fattr',
            [[ (Fm * BFILE.rep (FSXPBlockAlloc fsxp) (FSXPInode fsxp) flist')%pred (list2mem m') ]] *
            [[ (A * #inum |-> f')%pred (list2nmem flist') ]] *
            [[ bytes' = firstn newlen bytes ++ (repeat $0 (newlen - length bytes)) ]] *
-           [[ rep bytes' f' ]] *
-           [[ attr = INODE.Build_iattr ($ newlen) f.(BFILE.BFAttr).(INODE.IMTime) f.(BFILE.BFAttr).(INODE.IType) f.(BFILE.BFAttr).(INODE.IDev) ]] *
-           [[ f' = BFILE.Build_bfile fdata' attr ]])
+           [[ rep bytes' attr f' ]] *
+           [[ fattr' = INODE.Build_iattr ($ newlen) f.(BFILE.BFAttr).(INODE.IMTime) f.(BFILE.BFAttr).(INODE.IType) f.(BFILE.BFAttr).(INODE.IDev) ]] *
+           [[ f' = BFILE.Build_bfile fdata' fattr' ]])
        CRASH LOG.would_recover_old (FSXPLog fsxp) F mbase
      >} resize_file fsxp inum newlen mscs.
   Proof.
@@ -742,11 +750,11 @@ Module BYTEFILE.
     write_bytes fsxp inum off data mscs rx.
 
   Theorem append_ok: forall fsxp inum (off:nat) len (newbytes: bytes len) mscs,
-    {< m mbase F Fm Fi A flist f bytes,
+    {< m mbase F Fm Fi A flist f bytes attr,
       PRE LOG.rep (FSXPLog fsxp) F (ActiveTxn mbase m) mscs *
            [[ (Fm * BFILE.rep (FSXPBlockAlloc fsxp) (FSXPInode fsxp) flist)%pred (list2mem m) ]] *
            [[ (A * #inum |-> f)%pred (list2nmem flist) ]] *
-           [[ rep bytes f ]] *
+           [[ rep bytes attr f ]] *
            [[ Fi (list2nmem bytes) ]] *
            [[ goodSize addrlen (off + len) ]] *
            (* makes this an append *)
@@ -757,7 +765,7 @@ Module BYTEFILE.
            [[ ok = true ]] * exists flist' f' bytes' zeros,
            [[ (Fm * BFILE.rep (FSXPBlockAlloc fsxp) (FSXPInode fsxp) flist')%pred (list2mem m') ]] *
            [[ (A * #inum |-> f')%pred (list2nmem flist') ]] *
-           [[ rep bytes' f' ]] *
+           [[ rep bytes' attr f' ]] *
            [[ let newdata := @Rec.of_word (Rec.ArrayF byte_type len) newbytes in
               (Fi * zeros * arrayN off newdata)%pred (list2nmem bytes')]] *
            [[ zeros = arrayN (filelen f) (repeat $0 (off - (filelen f))) ]])
@@ -835,13 +843,13 @@ Module BYTEFILE.
 
   Hint Extern 1 ({{_}} progseq (append _ _ _ _ _) _) => apply append_ok : prog.
 
-  Theorem rep_unique : forall bytes1 bytes2 bf,
-    rep bytes1 bf -> rep bytes2 bf -> bytes1 = bytes2.
+  Theorem rep_unique : forall bytes1 bytes2 attr1 attr2 bf,
+    rep bytes1 attr1 bf -> rep bytes2 attr2 bf -> bytes1 = bytes2 /\ attr1 = attr2.
   Proof.
     unfold rep, bytes_rep; intros.
     repeat deex.
-    pose proof (array_item_file_eq H0 H).
-    congruence.
+    pose proof (array_item_file_eq H0 H); congruence.
+    destruct attr1; destruct attr2; simpl in *; congruence.
   Qed.
 
 End BYTEFILE.
